move edgep to sgraph

coq/extraction.v
@@ -141,43 +141,6 @@ Lemma uPathRP (G : sgraph) {A : pred G} x y : x != y ->
 Admitted. (* this is essentially upathPR *)
 
 
-(** TOTHINK: Providing an injection from (proofs of [x -- y]) to
-(trivial) paths and then using the monoid structure with [pcat] seems
-preferable to providing a cons operation *)
-
-Lemma edgep_proof (G : sgraph) (x y : G) (xy : x -- y) : 
-  spath x y [:: y]. 
-Proof. by rewrite spath_cons xy spathxx. Qed.
-
-Definition edgep (G : sgraph) (x y : G) (xy : x -- y) := 
-  Build_Path (edgep_proof xy).
-
-Lemma mem_edgep (G : sgraph) (x y z : G) (xy : x -- y) :
-  z \in edgep xy = (z == x) || (z == y).
-Proof. by rewrite mem_path !inE. Qed.
-
-Lemma splitL (G : sgraph) (x y : G) (p : Path x y) : 
-  x != y -> exists z xy (p' : Path z y), p = pcat (edgep xy) p' /\ p' =i tail p.
-Proof.
-  move => xy. case: p => p. elim: p x xy => [|a p IH] x xy H.
-  - move/spath_nil : (H) => ?. subst y. by rewrite eqxx in xy.
-  - move: (H) => H'. move: H. rewrite spath_cons => /andP [A B].
-    exists a. exists A. exists (Build_Path B). split; first exact: val_inj.
-    move => w. by rewrite in_collective nodesE !inE.
-Qed.
-
-Lemma splitR (G : sgraph) (x y : G) (p : Path x y) : 
-  x != y -> exists z (p' : Path x z) zy, p = pcat p' (edgep zy).
-Proof.
-  move => xy. case: p. elim/last_ind => [|p a IH] H.
-  - move/spath_nil : (H) => ?. subst y. by rewrite eqxx in xy.
-  - move: (H) => H'. 
-    case/andP : H. rewrite rcons_path => /andP [A B] C.
-    have sP : spath x (last x p) p by rewrite /spath A eqxx.
-    move: (spath_rcons H') => ?; subst a.
-    exists (last x p). exists (Build_Path sP). exists B. 
-    apply: val_inj => /=. by rewrite cats1.
-Qed.
 
 Lemma ins (T : finType) (A : pred T) x : x \in A -> x \in [set z in A].
 Proof. by rewrite inE. Qed.
